libcrux-ml-kem/src/vector/neon.rs
@@ -45,7 +45,15 @@ impl Operations for SIMD128Vector {
         add(lhs, rhs)
     }
 
+    fn add_opaque(lhs: Self, rhs: &Self) -> Self {
+        add(lhs, rhs)
+    }
+
     fn sub(lhs: Self, rhs: &Self) -> Self {
+        sub(lhs, rhs)
+    }
+
+    fn sub_opaque(lhs: Self, rhs: &Self) -> Self {
         sub(lhs, rhs)
     }
 
