libcrux-ml-kem/src/vector/traits.rs
@@ -15,6 +15,28 @@ pub trait Repr: Copy + Clone {
 
 #[cfg(not(eurydice))]
 #[hax_lib::attributes]
+#[hax_lib::fstar::before(interface,
+r#"[@@ "opaque_to_smt"]
+let sub_opaque_pre (lhs rhs: t_Array i16 (sz 16)) =
+    forall i. i < 16 ==>
+        Spec.Utils.is_intb (pow2 15 - 1) (v (Seq.index lhs i) - v (Seq.index rhs i))
+
+[@@ "opaque_to_smt"]
+let sub_opaque_post (lhs rhs result: t_Array i16 (sz 16)) =
+    forall i. i < 16 ==>
+        (v (Seq.index result i) == v (Seq.index lhs i) - v (Seq.index rhs i))"#
+)]
+#[hax_lib::fstar::before(interface,
+r#"[@@ "opaque_to_smt"]
+let add_opaque_pre (lhs rhs: t_Array i16 (sz 16)) =
+    forall i. i < 16 ==>
+        Spec.Utils.is_intb (pow2 15 - 1) (v (Seq.index lhs i) + v (Seq.index rhs i))
+
+[@@ "opaque_to_smt"]
+let add_opaque_post (lhs rhs result: t_Array i16 (sz 16)) =
+    forall i. i < 16 ==>
+        (v (Seq.index result i) == v (Seq.index lhs i) + v (Seq.index rhs i))"#
+)]
 pub trait Operations: Copy + Clone + Repr {
     #[allow(non_snake_case)]
     #[requires(true)]
@@ -37,12 +59,20 @@ pub trait Operations: Copy + Clone + Repr {
          v (Seq.index (f_repr ${lhs}) i) + v (Seq.index (f_repr ${rhs}) i))"#))]
     fn add(lhs: Self, rhs: &Self) -> Self;
 
+    #[requires(fstar!(r#"add_opaque_pre (f_repr ${lhs}) (f_repr ${rhs})"#))]
+    #[ensures(|result| fstar!(r#"add_opaque_post (f_repr ${lhs}) (f_repr ${rhs}) (f_repr ${result})"#))]
+    fn add_opaque(lhs: Self, rhs: &Self) -> Self;
+
     #[requires(fstar!(r#"forall i. i < 16 ==> 
         Spec.Utils.is_intb (pow2 15 - 1) (v (Seq.index (f_repr ${lhs}) i) - v (Seq.index (f_repr ${rhs}) i))"#))]
     #[ensures(|result| fstar!(r#"forall i. i < 16 ==> 
         (v (Seq.index (f_repr ${result}) i) == 
          v (Seq.index (f_repr ${lhs}) i) - v (Seq.index (f_repr ${rhs}) i))"#))]
     fn sub(lhs: Self, rhs: &Self) -> Self;
+
+    #[requires(fstar!(r#"sub_opaque_pre (f_repr ${lhs}) (f_repr ${rhs})"#))]
+    #[ensures(|result| fstar!(r#"sub_opaque_post (f_repr ${lhs}) (f_repr ${rhs}) (f_repr ${result})"#))]
+    fn sub_opaque(lhs: Self, rhs: &Self) -> Self;
 
     #[requires(fstar!(r#"forall i. i < 16 ==> 
         Spec.Utils.is_intb (pow2 15 - 1) (v (Seq.index (f_repr ${vec}) i) * v c)"#))]
