libcrux-ml-kem/proofs/fstar/extraction/Libcrux_ml_kem.Polynomial.fsti
@@ -62,62 +62,6 @@ let to_spec_matrix_t (#r:Spec.MLKEM.rank) (#v_Vector: Type0)
     (m:t_Array (t_Array (t_PolynomialRingElement v_Vector) r) r) : Spec.MLKEM.matrix r =
     createi r (fun i -> to_spec_vector_t #r #v_Vector (m.[i]))
 
-[@@ "opaque_to_smt"]
-let add_vector_pre (#v_Vector: Type0)
-      {| i1: Libcrux_ml_kem.Vector.Traits.t_Operations v_Vector |}
-      (lhs rhs: v_Vector) =
-    forall i. i < 16 ==>
-        Spec.Utils.is_intb (pow2 15 - 1) (v (Seq.index (Libcrux_ml_kem.Vector.Traits.f_to_i16_array lhs) i) +
-            v (Seq.index (Libcrux_ml_kem.Vector.Traits.f_to_i16_array rhs) i))
-
-[@@ "opaque_to_smt"]
-let add_vector_post (#v_Vector: Type0)
-      {| i1: Libcrux_ml_kem.Vector.Traits.t_Operations v_Vector |}
-      (result lhs rhs: v_Vector) =
-    forall i. i < 16 ==>
-        (v (Seq.index (Libcrux_ml_kem.Vector.Traits.f_to_i16_array result) i) == 
-            v (Seq.index (Libcrux_ml_kem.Vector.Traits.f_to_i16_array lhs) i) +
-                v (Seq.index (Libcrux_ml_kem.Vector.Traits.f_to_i16_array rhs) i))
-
-val add_vector
-      (#v_Vector: Type0)
-      {| i1: Libcrux_ml_kem.Vector.Traits.t_Operations v_Vector |}
-      (lhs rhs: v_Vector)
-    : Prims.Pure v_Vector
-      (requires add_vector_pre lhs rhs)
-      (ensures
-        fun result ->
-          let result:v_Vector = result in
-          add_vector_post result lhs rhs)
-
-[@@ "opaque_to_smt"]
-let sub_vector_pre (#v_Vector: Type0)
-      {| i1: Libcrux_ml_kem.Vector.Traits.t_Operations v_Vector |}
-      (lhs rhs: v_Vector) =
-    forall i. i < 16 ==>
-        Spec.Utils.is_intb (pow2 15 - 1) (v (Seq.index (Libcrux_ml_kem.Vector.Traits.f_to_i16_array lhs) i) -
-            v (Seq.index (Libcrux_ml_kem.Vector.Traits.f_to_i16_array rhs) i))
-
-[@@ "opaque_to_smt"]
-let sub_vector_post (#v_Vector: Type0)
-      {| i1: Libcrux_ml_kem.Vector.Traits.t_Operations v_Vector |}
-      (result lhs rhs: v_Vector) =
-    forall i. i < 16 ==>
-        (v (Seq.index (Libcrux_ml_kem.Vector.Traits.f_to_i16_array result) i) == 
-            v (Seq.index (Libcrux_ml_kem.Vector.Traits.f_to_i16_array lhs) i) -
-                v (Seq.index (Libcrux_ml_kem.Vector.Traits.f_to_i16_array rhs) i))
-
-val sub_vector
-      (#v_Vector: Type0)
-      {| i1: Libcrux_ml_kem.Vector.Traits.t_Operations v_Vector |}
-      (lhs rhs: v_Vector)
-    : Prims.Pure v_Vector
-      (requires sub_vector_pre lhs rhs)
-      (ensures
-        fun result ->
-          let result:v_Vector = result in
-          sub_vector_post result lhs rhs)
-
 [@@ FStar.Tactics.Typeclasses.tcinstance]
 val impl
       (#v_Vector: Type0)
@@ -164,10 +108,11 @@ val add_message_error_reduce
       (requires
         (forall (i: nat).
             i < 16 ==>
-            add_vector_pre myself.f_coefficients.[ sz i ] message.f_coefficients.[ sz i ] /\
+            Libcrux_ml_kem.Vector.Traits.f_add_opaque_pre myself.f_coefficients.[ sz i ]
+              message.f_coefficients.[ sz i ] /\
             Spec.Utils.is_i16b_array_opaque (28296 - 3328)
-              (Libcrux_ml_kem.Vector.Traits.f_to_i16_array (add_vector myself.f_coefficients.[ sz i
-                      ]
+              (Libcrux_ml_kem.Vector.Traits.f_to_i16_array (Libcrux_ml_kem.Vector.Traits.f_add_opaque
+                      myself.f_coefficients.[ sz i ]
                       message.f_coefficients.[ sz i ]))))
       (fun _ -> Prims.l_True)
 
@@ -179,9 +124,11 @@ val impl_2__add_message_error_reduce
       (requires
         (forall (i: nat).
             i < 16 ==>
-            add_vector_pre self.f_coefficients.[ sz i ] message.f_coefficients.[ sz i ] /\
+            Libcrux_ml_kem.Vector.Traits.f_add_opaque_pre self.f_coefficients.[ sz i ]
+              message.f_coefficients.[ sz i ] /\
             Spec.Utils.is_i16b_array_opaque (28296 - 3328)
-              (Libcrux_ml_kem.Vector.Traits.f_to_i16_array (add_vector self.f_coefficients.[ sz i ]
+              (Libcrux_ml_kem.Vector.Traits.f_to_i16_array (Libcrux_ml_kem.Vector.Traits.f_add_opaque
+                      self.f_coefficients.[ sz i ]
                       message.f_coefficients.[ sz i ]))))
       (fun _ -> Prims.l_True)
 
@@ -346,15 +293,16 @@ val add_to_ring_element
       (requires
         forall (i: nat).
           i < v (Core.Slice.impl__len myself.f_coefficients) ==>
-          add_vector_pre myself.f_coefficients.[ sz i ] rhs.f_coefficients.[ sz i ])
+          Libcrux_ml_kem.Vector.Traits.f_add_opaque_pre myself.f_coefficients.[ sz i ]
+            rhs.f_coefficients.[ sz i ])
       (ensures
         fun myself_future ->
           let myself_future:t_PolynomialRingElement v_Vector = myself_future in
           forall (i: nat).
             i < v (Core.Slice.impl__len myself.f_coefficients) ==>
-            add_vector_post myself_future.f_coefficients.[ sz i ]
-              myself.f_coefficients.[ sz i ]
-              rhs.f_coefficients.[ sz i ])
+            Libcrux_ml_kem.Vector.Traits.f_add_opaque_post myself.f_coefficients.[ sz i ]
+              rhs.f_coefficients.[ sz i ]
+              myself_future.f_coefficients.[ sz i ])
 
 /// Given two polynomial ring elements `lhs` and `rhs`, compute the pointwise
 /// sum of their constituent coefficients.
@@ -367,5 +315,6 @@ val impl_2__add_to_ring_element
       (requires
         forall (i: nat).
           i < v (Core.Slice.impl__len self.f_coefficients) ==>
-          add_vector_pre self.f_coefficients.[ sz i ] rhs.f_coefficients.[ sz i ])
+          Libcrux_ml_kem.Vector.Traits.f_add_opaque_pre self.f_coefficients.[ sz i ]
+            rhs.f_coefficients.[ sz i ])
       (fun _ -> Prims.l_True)
