libcrux-ml-kem/proofs/fstar/extraction/Libcrux_ml_kem.Vector.Traits.fsti
@@ -24,6 +24,26 @@ class t_Repr (v_Self: Type0) = {
     -> Prims.Pure (t_Array i16 (sz 16)) (f_repr_pre x0) (fun result -> f_repr_post x0 result)
 }
 
+[@@ "opaque_to_smt"]
+let add_opaque_pre (lhs rhs: t_Array i16 (sz 16)) =
+    forall i. i < 16 ==>
+        Spec.Utils.is_intb (pow2 15 - 1) (v (Seq.index lhs i) + v (Seq.index rhs i))
+
+[@@ "opaque_to_smt"]
+let add_opaque_post (lhs rhs result: t_Array i16 (sz 16)) =
+    forall i. i < 16 ==>
+        (v (Seq.index result i) == v (Seq.index lhs i) + v (Seq.index rhs i))
+
+[@@ "opaque_to_smt"]
+let sub_opaque_pre (lhs rhs: t_Array i16 (sz 16)) =
+    forall i. i < 16 ==>
+        Spec.Utils.is_intb (pow2 15 - 1) (v (Seq.index lhs i) - v (Seq.index rhs i))
+
+[@@ "opaque_to_smt"]
+let sub_opaque_post (lhs rhs result: t_Array i16 (sz 16)) =
+    forall i. i < 16 ==>
+        (v (Seq.index result i) == v (Seq.index lhs i) - v (Seq.index rhs i))
+
 class t_Operations (v_Self: Type0) = {
   [@@@ FStar.Tactics.Typeclasses.no_method]_super_13011033735201511749:Core.Marker.t_Copy v_Self;
   [@@@ FStar.Tactics.Typeclasses.no_method]_super_9529721400157967266:Core.Clone.t_Clone v_Self;
@@ -72,6 +92,12 @@ class t_Operations (v_Self: Type0) = {
                 v (Seq.index (f_repr lhs) i) + v (Seq.index (f_repr rhs) i))) };
   f_add:x0: v_Self -> x1: v_Self
     -> Prims.Pure v_Self (f_add_pre x0 x1) (fun result -> f_add_post x0 x1 result);
+  f_add_opaque_pre:lhs: v_Self -> rhs: v_Self
+    -> pred: Type0{add_opaque_pre (f_repr lhs) (f_repr rhs) ==> pred};
+  f_add_opaque_post:lhs: v_Self -> rhs: v_Self -> result: v_Self
+    -> pred: Type0{pred ==> add_opaque_post (f_repr lhs) (f_repr rhs) (f_repr result)};
+  f_add_opaque:x0: v_Self -> x1: v_Self
+    -> Prims.Pure v_Self (f_add_opaque_pre x0 x1) (fun result -> f_add_opaque_post x0 x1 result);
   f_sub_pre:lhs: v_Self -> rhs: v_Self
     -> pred:
       Type0
@@ -90,6 +116,12 @@ class t_Operations (v_Self: Type0) = {
                 v (Seq.index (f_repr lhs) i) - v (Seq.index (f_repr rhs) i))) };
   f_sub:x0: v_Self -> x1: v_Self
     -> Prims.Pure v_Self (f_sub_pre x0 x1) (fun result -> f_sub_post x0 x1 result);
+  f_sub_opaque_pre:lhs: v_Self -> rhs: v_Self
+    -> pred: Type0{sub_opaque_pre (f_repr lhs) (f_repr rhs) ==> pred};
+  f_sub_opaque_post:lhs: v_Self -> rhs: v_Self -> result: v_Self
+    -> pred: Type0{pred ==> sub_opaque_post (f_repr lhs) (f_repr rhs) (f_repr result)};
+  f_sub_opaque:x0: v_Self -> x1: v_Self
+    -> Prims.Pure v_Self (f_sub_opaque_pre x0 x1) (fun result -> f_sub_opaque_post x0 x1 result);
   f_multiply_by_constant_pre:vec: v_Self -> c: i16
     -> pred:
       Type0
